Show Schreier.sound_build up to compose_generator.

B4_group.v
@@ -19,7 +19,7 @@ Notation Canonical := (Pruned xH).
 Variable gen : list perm.
 
 (* A permutation can be composed from the generating set. *)
-Definition Generates π := ∃w, w ⊆ gen /\ can π = compose' w.
+Definition Generates π := ∃w, w ⊆ gen /\ can π = can (compose' w).
 
 (* The number of distinct permutations that are generated. *)
 Record Group_Order (ord : positive) := Group_Order_Witness {
@@ -28,6 +28,18 @@ Record Group_Order (ord : positive) := Group_Order_Witness {
   enum_surjective : ∀π, Generates π -> ∃i, i <= ord /\ enum i = can π;
   enum_injective : ∀i j, i <= ord -> j <= ord -> enum i = enum j -> i = j;
 }.
+
+(***
+Theorems
+*)
+
+Theorem compose_generator σ π :
+  Generates π -> In σ gen -> Generates (σ ∘ π).
+Proof.
+intros [w []] ?; exists (w ++ [σ]); split.
+apply incl_app. easy. apply incl_cons; [easy|apply incl_nil_l].
+rewrite fold_left_app; simpl.
+Admitted.
 
 End Groups.
 
