A1_setup.v
@@ -30,21 +30,27 @@ Notation "opt ?? d" :=
 (******************************************************************************)
 
 Ltac inv H := inversion H; subst; clear H; try easy.
+Ltac simple_ind x := induction x; simpl; intros; [easy|].
 
 Ltac convert_bool_once :=
   match goal with
   | [H : _ && _ = true |- _] =>  apply andb_prop in H; destruct H
   | [H : _ || _ = true |- _]  => apply orb_true_elim in H; destruct H
   | [H : _ || _ = false |- _]  => apply orb_false_elim in H; destruct H
+  | |- (_ && _ = true)   => apply andb_true_intro; split
+  | |- (_ || _ = false)  => apply orb_false_intro
+  | |- (_ || _ = true)   => apply orb_true_intro
+  | _ => idtac
+  end.
+
+Ltac convert_Nat_bool_once :=
+  match goal with
   | [H : _ =? _ = true |- _]   => apply Nat.eqb_eq in H
   | [H : _ =? _ = false |- _]  => apply Nat.eqb_neq in H
   | [H : _ <=? _ = true |- _]  => apply Nat.leb_le in H
   | [H : _ <=? _ = false |- _] => apply Nat.leb_gt in H
   | [H : _ <? _ = true |- _]   => apply Nat.ltb_lt in H
   | [H : _ <? _ = false |- _]  => apply Nat.ltb_ge in H
-  | |- (_ && _ = true)   => apply andb_true_intro; split
-  | |- (_ || _ = false)  => apply orb_false_intro
-  | |- (_ || _ = true)   => apply orb_true_intro
   | |- (_ =? _ = true)   => apply Nat.eqb_eq
   | |- (_ =? _ = false)  => apply Nat.eqb_neq
   | |- (_ <=? _ = true)  => apply Nat.leb_le
@@ -54,7 +60,27 @@ Ltac convert_bool_once :=
   | _ => idtac
   end.
 
-Ltac convert_bool := repeat convert_bool_once.
+Ltac convert_Pos_bool_once :=
+  match goal with
+  | [H : _ =? _ = true |- _]   => apply Pos.eqb_eq in H
+  | [H : _ =? _ = false |- _]  => apply Pos.eqb_neq in H
+  | [H : _ <=? _ = true |- _]  => apply Pos.leb_le in H
+  | [H : _ <=? _ = false |- _] => apply Pos.leb_gt in H
+  | [H : _ <? _ = true |- _]   => apply Pos.ltb_lt in H
+  | [H : _ <? _ = false |- _]  => apply Pos.ltb_ge in H
+  | |- (_ =? _ = true)   => apply Pos.eqb_eq
+  | |- (_ =? _ = false)  => apply Pos.eqb_neq
+  | |- (_ <=? _ = true)  => apply Pos.leb_le
+  | |- (_ <=? _ = false) => apply Pos.leb_gt
+  | |- (_ <? _ = true)   => apply Pos.ltb_lt
+  | |- (_ <? _ = false)  => apply Pos.ltb_ge
+  | _ => idtac
+  end.
+
+Ltac convert_bool :=
+  repeat convert_bool_once;
+  repeat convert_Nat_bool_once;
+  repeat convert_Pos_bool_once.
 
 Lemma wd {X Y} (f : X -> Y) x x' :
   x = x' -> f x = f x'.
