C1_Schreier_vector.v
@@ -54,8 +54,7 @@ Variable k : positive.
 
 (* Build an orbit vector given an orbit size bound. *)
 (* Note that it doesn't make a difference if the bound is bigger than needed. *)
-Definition build (bound : nat) :=
-  loop (insert Leaf k ident) [k] bound.
+Definition build (bound : nat) := loop (insert Leaf k ident) [k] bound.
 
 (* The orbit given by they keys of the Schreier vector. *)
 Definition orbit (V : vector) : list positive := map fst (entries V xH).
@@ -70,7 +69,7 @@ Definition generators (V : vector) : list perm :=
 Theorems
 *)
 
-Section Schreiers_lemma.
+Section Soundness.
 
 (* The orbit permutations are valid. *)
 Definition Sound (V : vector) := ∀i,
@@ -79,18 +78,62 @@ Definition Sound (V : vector) := ∀i,
   | None => True
   end.
 
-(* The vector contains the full orbit. *)
-Definition Complete (V : vector) := ∀π, Generates gen π -> lookup V π⋅k ≠ None.
+Lemma sound_extend h gen' V acc :
+  Generates gen h -> gen' ⊆ gen ->
+  Sound V -> Sound (fst (extend h⋅k h gen' V acc)).
+Proof.
+revert V acc; simple_ind gen'.
+apply incl_cons_inv in H0 as [].
+destruct (lookup _); apply IHgen'; try easy.
+intros j; rewrite lookup_insert.
+destruct (_ =? _) eqn:E; [convert_bool; subst; split|apply H1].
+apply compose_generator; easy. apply apply_compose.
+Qed.
+
+Lemma sound_extend_loop V try acc :
+  Sound V -> Sound (fst (extend_loop V try acc)).
+Proof.
+revert V acc; simple_ind try.
+destruct (lookup V a) eqn:E. destruct (extend _) as [V' acc'] eqn:E'.
+replace V' with (fst (extend a p gen V acc)) by (rewrite E'; easy).
+all: apply IHtry. assert(Ha := H a); rewrite E in Ha; destruct Ha; subst.
+apply sound_extend; easy. easy.
+Qed.
+
+Lemma sound_loop V try n :
+  Sound V -> Sound (loop V try n).
+Proof.
+revert V try; simple_ind n.
+destruct (extend_loop V _) as [V' try'] eqn:E.
+replace V' with (fst (extend_loop V try [])) by (rewrite E; easy).
+destruct try'. apply sound_extend_loop, H.
+apply IHn, sound_extend_loop, H.
+Qed.
 
 Theorem sound_build bound :
   Sound (build bound).
 Proof.
-Admitted.
+apply sound_loop.
+intros i. rewrite lookup_insert; simpl.
+destruct (k =? i) eqn:E. convert_bool; subst.
+split. exists []; simpl; easy. easy. easy.
+Qed.
+
+End Soundness.
+
+Section Completeness.
+
+(* The vector contains the full orbit. *)
+Definition Complete (V : vector) := ∀π, Generates gen π -> lookup V π⋅k ≠ None.
 
 Theorem complete_build bound :
   (size (union_range gen) <= bound)%nat -> Complete (build bound).
 Proof.
 Admitted.
+
+End Completeness.
+
+Section Schreiers_lemma.
 
 Variable V : vector.
 Hypothesis sound : Sound V.
